Update test files

Source/IntegrationTests/TestFiles/LitTests/LitTest/traits/TraitCompileErrors.dfy
@@ -4,17 +4,10 @@
 module StaticMembers {
   trait Tr {
     // the following static members must also be given bodies, but that's checked by the compiler
-<<<<<<< HEAD:Test/traits/TraitCompileErrors.dfy
-    static function method Func(): int ensures false
+    static ghost function Func(): int ensures false
     static method Method() ensures false
     static twostate function TwoF(): int ensures false
     static twostate lemma TwoL() ensures false
-=======
-    static ghost function Func(): int
-    static method Method()
-    static twostate function TwoF(): int
-    static twostate lemma TwoL()
->>>>>>> origin/master:Source/IntegrationTests/TestFiles/LitTests/LitTest/traits/TraitCompileErrors.dfy
     static least predicate P()
     static greatest predicate Q()
     static least lemma IL() ensures false
