Source/IntegrationTests/TestFiles/LitTests/LitTest/irondafny0/opened_workaround.dfy
@@ -3,21 +3,12 @@
 
 module A {
 
-<<<<<<< HEAD:Test/irondafny0/opened_workaround.dfy
-    predicate P() ensures false
+    ghost predicate P() ensures false
 
     class C
     {
-        static ghost method{:axiom} M()
-            ensures P();
-=======
-    ghost predicate P()
-
-    class C
-    {
-        static method{:axiom} M()
+        static ghost method {:axiom} M()
             ensures P()
->>>>>>> origin/master:Source/IntegrationTests/TestFiles/LitTests/LitTest/irondafny0/opened_workaround.dfy
     }
 }
 
