docs/DafnyRef/GrammarDetails.md
@@ -1046,13 +1046,9 @@ AssertStmt =
   )
 ````
 
-<<<<<<< HEAD
-#### 17.2.6.17. assume statement ([discussion](#sec-assume-statement)) {#g-assume-statement}
-=======
 #### 17.2.6.17. Assume statement {#g-assume-statement}
 
 ([discussion](#sec-assume-statement)) 
->>>>>>> origin/master
 
 ````grammar
 AssumeStmt =
